\documentclass[a4paper]{amsart}
\usepackage{a4wide}
\usepackage[]{graphicx}

\setlength{\parindent}{0.0in}
\setlength{\parskip}{0.1in}

\newcommand{\laplace}[1]{\mathcal{L}\{#1\}}
\newcommand{\Hv}{\textrm{H}}
\renewcommand{\b}{\mathbf}

\begin{document}
\title{6G5Z3011 Multi-variable calculus and analytical methods}
\author{Tutorial Sheet 7}
\maketitle

\textbf{Qs 1 -- 5} on working with the Laplace transform and its inverse. \\
\textbf{Qs 6 -- 7} on solving ODEs and systems of ODEs using the Laplace transform method. 
\begin{enumerate}
    \item 
    Find the general solution of the equation
    $$ \frac{d^3y}{dx^3} = 6 .$$
    
    What does the solution become if we are given the conditions 
    $$y(0)=0, \quad y(1)=0, \quad y(2)=1 ?$$
    
    \item
    Using the fact that 
    $$ \sinh{t} = \frac{1}{2} \left ( e^t -e^{-t} \right ) $$
    and the definition of the Laplace transform show that
    $$\laplace{\sinh{at}}  = \frac{a}{s^2 - a^2} .$$
    
    \item
    Without using the tables (i.e. by working the integral definition of the transform) show that 
    $$ \laplace{ t^2 } = \dfrac{2}{s^3}.$$
    
    \item
    Using the table of standard transforms and transform properties find the Laplace transforms of the functions defined by
    \begin{enumerate}
    \item
    $$1 + 2t + 3t^2 ,$$
    \item
    $$5\cos{t} ,$$
    \item
    $$4e^{2t}\sin{3t} .$$
    \end{enumerate}
    
    \item
    Using the table find the inverse Laplace transforms of
    \begin{enumerate}
    \item
    $$\dfrac{7}{s+4} ,$$
    \item
    $$\dfrac{4s + 3}{s^2} ,$$
    \item
    $$\dfrac{2s+8}{(s+4)^2 + 100} ,$$
    \item
    $$\dfrac{3}{(s+1)(s-2)} .$$
    \end{enumerate}
    \item
Use the Laplace transform method to solve the following differential equations subject to the given initial conditions

\begin{enumerate}
\item
$$\frac{dy}{dt} + y = 1, \quad y(0)=0 .$$

\item
$$\frac{dy}{dt} - 2y = 4 e^{-2t}, \quad y(0)=2.$$

\item
$$\frac{d^2y}{dt^2} + 2y = 3t, \quad y(0)=1, \, y'(0)=7.$$

\item
$$\frac{d^2y}{dt^2} +2 \frac{dy}{dt} + y = 3, \quad y(0)=1, \, y'(0)=4.$$
\end{enumerate}

\bigskip

\item
Use the Laplace transform method to solve the following pairs of coupled differential equations.

\begin{enumerate}
\item
\begin{align*}
x + \frac{dy}{dt} &=2 \\
\frac{dx}{dt} -6x - 13 y &=1
\end{align*}
with the initial conditions $x(0)=-10$ and $y(0)=3$.

\item
\begin{align*}
\frac{d^2y}{dt^2} + 2 \frac{dx}{dt} + y &=0 \\
\frac{dy}{dt} - \frac{dx}{dt} - 2y + 2x &= \sin t.
\end{align*}
with the initial conditions $x(0)=0$, $y(0)=0$ and $y'(0)=0$.	
\end{enumerate}


\end{enumerate}

\end{document}